fix tests

Diff_Arr.thy
@@ -8,40 +8,40 @@ begin
 
 type_synonym 'a diff_arr = "'a cell ref"
 
-qualified definition from_array :: "('a::heap) array \<Rightarrow> 'a diff_arr Heap" where
+qualified definition from_array :: 
+  "('a::heap) array \<Rightarrow> 'a diff_arr Heap" 
+where
   "from_array a = do {
     ref (Array a)
   }"
 
-qualified definition from_list :: "('a::heap) list \<Rightarrow> 'a diff_arr Heap" where
+qualified definition from_list :: 
+  "('a::heap) list \<Rightarrow> 'a diff_arr Heap" 
+where
   "from_list xs = do {
     a \<leftarrow> Array.of_list xs;
     from_array a
   }"
 
-qualified partial_function (heap) lookup :: "('a::heap) diff_arr \<Rightarrow> nat \<Rightarrow> 'a Heap" where
-  "lookup diff_arr n = do {
+qualified partial_function (heap) lookup :: 
+  "('a::heap) diff_arr \<Rightarrow> nat \<Rightarrow> 'a Heap" 
+where
+  "lookup diff_arr i = do {
       cell \<leftarrow> !diff_arr;
       case cell of
-        Array array   \<Rightarrow> Array.nth array n
-      | Upd m value r \<Rightarrow> if n = m 
-                         then return value
-                         else lookup r n
+        Array array            \<Rightarrow>
+          Array.nth array i
+      | Upd i' value diff_arr' \<Rightarrow>
+          if i = i'
+          then return value
+          else lookup diff_arr' i
   }"
 declare lookup.simps[code]
 
-(* TODO: Use size type class *)
-qualified partial_function (heap) length :: "('a::heap) diff_arr \<Rightarrow> nat Heap" where
-  "length diff_arr = do {
-      cell \<leftarrow> !diff_arr;
-      case cell of
-        Array array   \<Rightarrow> Array.len array
-      | Upd m value r \<Rightarrow> length r
-  }"
-declare length.simps[code]
-
 (* TODO: use array_copy? *)
-qualified partial_function (heap) realize :: "('a::heap) diff_arr \<Rightarrow> 'a array Heap" where
+qualified partial_function (heap) realize :: 
+  "('a::heap) diff_arr \<Rightarrow> 'a array Heap" 
+where
   "realize diff_arr = do {
     cell \<leftarrow> !diff_arr;
      case cell of
@@ -56,6 +56,25 @@ qualified partial_function (heap) realize :: "('a::heap) diff_arr \<Rightarrow> 
         }
   }"
 declare realize.simps[code]
+
+abbreviation update_if_none where
+  "update_if_none m i v \<equiv> (case m i of None \<Rightarrow> m(i \<mapsto> v) | Some _ \<Rightarrow> m)"
+
+(* Tailrec version, ask Peter if this makes sense *)
+qualified partial_function (heap) realize' :: 
+  "('a::heap) diff_arr \<Rightarrow> (nat \<rightharpoonup> 'a) \<Rightarrow> 'a array Heap" 
+where
+  "realize' diff_arr upds = do {
+    cell \<leftarrow> !diff_arr;
+     case cell of
+        Array arr \<Rightarrow> do {
+            len \<leftarrow> Array.len arr;
+            xs  \<leftarrow> Array.freeze arr;
+            Array.make len (\<lambda>i. case upds i of None \<Rightarrow> List.nth xs i | Some v \<Rightarrow> v)
+        }
+      | Upd i v diff_arr \<Rightarrow> realize' diff_arr (update_if_none upds i v)
+  }"
+declare realize'.simps[code]
 
 qualified partial_function (heap) update :: 
     "('a::heap) diff_arr \<Rightarrow> nat \<Rightarrow> 'a::heap \<Rightarrow> 'a diff_arr Heap"
@@ -78,10 +97,41 @@ where
   }"
 declare update.simps[code]
 
+qualified partial_function (heap) update' :: 
+    "('a::heap) diff_arr \<Rightarrow> nat \<Rightarrow> 'a::heap \<Rightarrow> 'a diff_arr Heap"
+where
+  "update' diff_arr i v = do {
+      cell \<leftarrow> !diff_arr;
+      case cell of
+        Array arr \<Rightarrow> do {
+          new_diff_arr \<leftarrow> ref (Array arr);
+          old_v \<leftarrow> Array.nth arr i;
+          diff_arr :=\<^sub>R Upd i old_v new_diff_arr;
+          Array.upd i v arr;
+          return new_diff_arr
+        }
+      | Upd _ _ _ \<Rightarrow> do {
+          arr \<leftarrow> realize' diff_arr Map.empty;
+          Array.upd i v arr;
+          ref (Array arr) 
+        }
+  }"
+
+qualified partial_function (heap) length :: 
+  "('a::heap) diff_arr \<Rightarrow> nat Heap" 
+where
+  "length diff_arr = do {
+      cell \<leftarrow> !diff_arr;
+      case cell of
+        Array array   \<Rightarrow> Array.len array
+      | Upd m value r \<Rightarrow> length r
+  }"
+declare length.simps[code]
+
 end
 
-lemma ref_lookup_upd: "\<lbrakk>t \<turnstile> xs \<sim>\<^sub>n a; 0 < n\<rbrakk>
-   \<Longrightarrow> <master_assn t> !a <\<lambda>c. master_assn t * \<up>(\<exists>x y z. c = Upd x y z)>"
+lemma ref_lookup_upd: "\<lbrakk>t \<turnstile> xs \<sim>\<^sub>n a; 0 < n\<rbrakk> \<Longrightarrow> 
+  <master_assn t> !a <\<lambda>c. master_assn t * \<up>(\<exists>x y z. c = Upd x y z)>"
 proof(induction n)
   case 0
   then show ?case
@@ -123,10 +173,10 @@ lemma from_list [sep_heap_rules]:
   "<emp> Diff_Arr.from_list xs <\<lambda>r. \<exists>\<^sub>At. master_assn t * \<up>(t \<turnstile> xs \<sim> r)>"
   by(sep_auto simp: Let_def)
 
-lemma lookup_aux: "
-  <\<up>(t \<turnstile> xs \<sim>\<^sub>n a \<and> i < length xs) * master_assn t >
+lemma lookup_aux: 
+  "<\<up>(t \<turnstile> xs \<sim>\<^sub>n a \<and> i < length xs) * master_assn t >
       Diff_Arr.lookup a i 
-  <\<lambda>r. master_assn t * \<up>(r = xs!i)>"
+   <\<lambda>r. master_assn t * \<up>(r = xs!i)>"
 proof(induction n arbitrary: xs a)
   case 0
   then show ?case 
@@ -143,10 +193,10 @@ next
     by(sep_auto simp: close_master_assn_upd')
 qed
 
-lemma lookup [sep_heap_rules]: "
-  <master_assn t * \<up>(t \<turnstile> xs \<sim> a \<and> i < length xs)> 
+lemma lookup [sep_heap_rules]: 
+  "<master_assn t * \<up>(t \<turnstile> xs \<sim> a \<and> i < length xs)> 
      Diff_Arr.lookup a i 
-  <\<lambda>r. master_assn t * \<up>(r = xs!i)>"
+   <\<lambda>r. master_assn t * \<up>(r = xs!i)>"
   unfolding diff_arr_rel_def
   using lookup_aux[of t]
   by sep_auto
@@ -179,6 +229,46 @@ next
     by sep_auto
 qed
 
+lemma helper: "i < length xs' \<Longrightarrow>
+  (case (case upds i of None \<Rightarrow> upds(i \<mapsto> x) | Some x \<Rightarrow> upds) i' of 
+     None \<Rightarrow> xs' ! i'
+   | Some v \<Rightarrow> v) = 
+  (case upds i' of None \<Rightarrow> xs'[i := x] ! i' | Some v \<Rightarrow> v)"
+  by(auto simp: nth_list_update split: option.splits)
+
+lemma realize'_aux: 
+ "<master_assn t * \<up>(t \<turnstile> xs \<sim>\<^sub>n diff_arr)> 
+     Diff_Arr.realize' diff_arr upds
+  <\<lambda>arr. master_assn t * arr \<mapsto>\<^sub>a 
+        (map (\<lambda>i. case upds i of None \<Rightarrow> xs ! i | Some v \<Rightarrow> v) [0..<length xs])>" 
+proof(induction n arbitrary: t diff_arr xs upds)
+  case 0
+  then show ?case
+    apply sep_auto
+    apply(subst realize'.simps)
+    apply(sep_drule r: open_master_assn)
+    apply sep_auto
+    apply(sep_drule r: close_master_assn_array)
+    by(sep_auto simp: map_nth)
+next
+  case (Suc n)
+  then show ?case
+    apply sep_auto
+    apply(subst realize'.simps)
+    apply(sep_drule r: open_master_assn)
+    apply sep_auto
+    apply(sep_drule r: close_master_assn_upd)
+    apply(sep_auto)
+    apply(sep_drule r: open_master_assn)
+    apply sep_auto
+    apply(sep_drule r: close_master_assn_upd)
+    apply sep_auto
+    subgoal for i x a' xs'
+      using Suc[of t xs' a' "(case upds i of None \<Rightarrow> upds(i \<mapsto> x) | Some x \<Rightarrow> upds)"]
+      by(sep_auto simp: helper)
+    done
+qed
+
 lemma realize [sep_heap_rules]: 
   "<master_assn t * \<up>(t \<turnstile> xs \<sim> diff_arr)> 
      Diff_Arr.realize diff_arr
@@ -186,6 +276,14 @@ lemma realize [sep_heap_rules]:
   unfolding diff_arr_rel_def
   using realize_aux[of t]
   by sep_auto
+
+lemma realize' [sep_heap_rules]: 
+  "<master_assn t * \<up>(t \<turnstile> xs \<sim> diff_arr)> 
+     Diff_Arr.realize' diff_arr Map.empty
+   <\<lambda>arr. master_assn t * arr \<mapsto>\<^sub>a xs>" 
+  unfolding diff_arr_rel_def
+  using realize'_aux[of t xs _ diff_arr Map.empty]
+  by(sep_auto simp: map_nth)
 
 lemma update_diff_arr_rel: "\<lbrakk>
   i < length xs; 
@@ -282,6 +380,46 @@ next
    done
 qed
 
+lemma update'_aux: 
+  assumes
+    "i < length xs"
+    "t \<turnstile> xs \<sim>\<^sub>n diff_arr"
+  shows
+    "<master_assn t> 
+       Diff_Arr.update' diff_arr i v
+     <\<lambda>diff_arr. \<exists>\<^sub>At'. master_assn t' * 
+       \<up>((\<forall>xs' diff_arr'. t \<turnstile> xs' \<sim> diff_arr' \<longrightarrow> t' \<turnstile> xs' \<sim> diff_arr') \<and> 
+         (t' \<turnstile> xs[i := v] \<sim> diff_arr))>"
+proof(cases "n = 0")
+  case True
+  with assms show ?thesis
+      unfolding diff_arr_rel_def
+      apply(simp add: update'.simps)
+      apply(hoare_triple_preI rule: master_assn_distinct)
+      apply(sep_drule r: open_master_assn)
+      apply(sep_auto eintros del: exI)       
+      subgoal for new_arr new_diff_arr
+        apply(rule exI[where x = 
+                     "(new_diff_arr, Array' (xs[i := v])) #
+                      (diff_arr, Upd' i (xs ! i) new_diff_arr) #
+                      (remove1 (diff_arr, Array' xs) t)"
+                ]) 
+        by(sep_auto simp: update_diff_arr_rel open_master_assn_cons exI[where x = 0])
+      done
+next
+  case False
+  with realize'_aux[of t xs n diff_arr Map.empty] assms show ?thesis
+  unfolding diff_arr_rel_def
+  apply(subst update'.simps)
+  apply(sep_auto heap: ref_lookup_upd eintros del: exI)
+  subgoal for new_arr new_diff_arr
+    apply(rule exI[where x = "(new_diff_arr, Array' (xs[i := v])) #  t"])
+    by(sep_auto simp: 
+        map_nth diff_arr_rel'_cons' exI[where x = 0] open_master_assn_cons[of new_diff_arr]
+       )
+   done
+qed
+
 lemma update[sep_heap_rules]: 
   "<master_assn t * \<up>(t \<turnstile> xs \<sim> diff_arr \<and> i < length xs)> 
      Diff_Arr.update diff_arr i v
@@ -289,6 +427,14 @@ lemma update[sep_heap_rules]:
     \<up>((\<forall>xs' diff_arr'. t \<turnstile> xs' \<sim> diff_arr' \<longrightarrow> t' \<turnstile> xs' \<sim> diff_arr') \<and> 
       (t' \<turnstile> xs[i := v] \<sim> diff_arr))>"
   by(sep_auto heap: update_aux simp: diff_arr_rel_def)
+
+lemma update'[sep_heap_rules]: 
+  "<master_assn t * \<up>(t \<turnstile> xs \<sim> diff_arr \<and> i < length xs)> 
+     Diff_Arr.update' diff_arr i v
+   <\<lambda>diff_arr. \<exists>\<^sub>At'. master_assn t' * 
+    \<up>((\<forall>xs' diff_arr'. t \<turnstile> xs' \<sim> diff_arr' \<longrightarrow> t' \<turnstile> xs' \<sim> diff_arr') \<and> 
+      (t' \<turnstile> xs[i := v] \<sim> diff_arr))>"
+  by(sep_auto heap: update'_aux simp: diff_arr_rel_def)
 
 lemma length_aux: "t \<turnstile> xs \<sim>\<^sub>n diff_arr \<Longrightarrow> 
   <master_assn t> 
@@ -310,10 +456,10 @@ next
     by(sep_auto simp: close_master_assn_upd')
 qed
 
-lemma length[sep_heap_rules]: "
-  <master_assn t * \<up>(t \<turnstile> xs \<sim> diff_arr)> 
-    Diff_Arr.length diff_arr
-  <\<lambda>len. master_assn t * \<up>(len = length xs)>"
+lemma length [sep_heap_rules]: 
+  "<master_assn t * \<up>(t \<turnstile> xs \<sim> diff_arr)> 
+     Diff_Arr.length diff_arr
+   <\<lambda>len. master_assn t * \<up>(len = length xs)>"
   unfolding diff_arr_rel_def
   by(sep_auto heap: length_aux)
 
