Diff_Arr_Safe.thy
@@ -21,7 +21,27 @@ qualified definition update where
     else return arr
   }"
 
+qualified definition update' where
+  "update' arr i v = do {
+    len \<leftarrow> Diff_Arr.length arr;
+    if i < len
+    then Diff_Arr.update' arr i v 
+    else return arr
+  }"
+
 end
+
+lemma lookup_safe [sep_heap_rules]: "
+  <master_assn t * \<up>(t \<turnstile> xs \<sim> a)> 
+     Diff_Arr_Safe.lookup a i 
+  <\<lambda>r. master_assn t * \<up>(r = xs!i)>"
+  unfolding Diff_Arr_Safe.lookup_def
+  apply sep_auto
+  using length 
+  apply sep_auto
+  apply sep_auto
+  using lookup
+  by(sep_auto simp: nth_undefined[of xs i])+
 
 lemma update_safe [sep_heap_rules]: "
   <master_assn t * \<up>(t \<turnstile> xs \<sim> diff_arr)> 
@@ -37,16 +57,18 @@ lemma update_safe [sep_heap_rules]: "
   apply(rule fi_rule[OF update, where F = emp])
   by sep_auto+
 
-lemma lookup_safe [sep_heap_rules]: "
-  <master_assn t * \<up>(t \<turnstile> xs \<sim> a)> 
-     Diff_Arr_Safe.lookup a i 
-  <\<lambda>r. master_assn t * \<up>(r = xs!i)>"
-  unfolding Diff_Arr_Safe.lookup_def
+lemma update'_safe [sep_heap_rules]: "
+  <master_assn t * \<up>(t \<turnstile> xs \<sim> diff_arr)> 
+     Diff_Arr_Safe.update' diff_arr i v
+  <\<lambda>diff_arr. \<exists>\<^sub>At'. master_assn t' * 
+    \<up>((\<forall>xs' diff_arr'. t \<turnstile> xs' \<sim> diff_arr' \<longrightarrow> t' \<turnstile> xs' \<sim> diff_arr') 
+      \<and> (t' \<turnstile> xs[i := v] \<sim> diff_arr))>"
+  unfolding Diff_Arr_Safe.update'_def
   apply sep_auto
-  using length 
-  apply sep_auto
-  apply sep_auto
-  using lookup
-  by(sep_auto simp: nth_undefined[of xs i])+
+  apply(rule fi_rule[OF length, where F = emp])
+  apply sep_auto+
+  apply(rule cons_post_rule)
+  apply(rule fi_rule[OF update', where F = emp])
+  by sep_auto+
 
 end
