Test_Hnr.thy
@@ -51,7 +51,7 @@ definition if_2 where
          t1 = if xs = [] 
               then xs 
               else let t1 = xs[c1 := c1]; 
-                       t2 = t1[c1:= c1] 
+                       t2 = t1[c1 := c1] 
                    in t2 
       in t1)"
 
@@ -97,233 +97,228 @@ definition if_7 where
             in (t1, t1)
     )"
 
+definition tuple_list where
+  "tuple_list xs = (let c1 = 1; c2 = (c1, c1); t1 = xs[c1 := c2] in t1)"
 
-
-definition test where
-  "test xs = (let c1 = 1; c2 = (c1, c1); t1 = xs[c1 := c2] in t1)"
-
-definition test_2 where
-  "test_2 xs = (let c1 = 1; t1 = xs[c1 := c1] in if_7 t1)"
+definition nested where
+  "nested xs = (let c1 = 1; t1 = xs[c1 := c1] in sequential_1 t1)"
 
 definition fallback_1 where
   "fallback_1 xs = 
     (let c1 = 1; b = (c1 = c1); t1 = if b then xs else xs[c1 := c1] in t1)"
 
 definition create_list where
-  "create_list x = [x]" 
+  "create_list x = (let xs = [x] in xs)" 
 
 definition create_arr where
-  "create_arr xs = New_Arr [xs]"
+  "create_arr xs = (let a = New_Arr xs in a)"
 
-definition create_diff_arr_empty where
+definition create_arr_2 where
+  "create_arr_2 x = New_Arr [x]"
+
+definition create_diff_arr_empty :: "('a::heap) list" where
   "create_diff_arr_empty = New_Diff_Arr []" 
 
-definition create_diff_arr where
+definition create_diff_arr :: "'a::heap \<Rightarrow> 'a list" where
   "create_diff_arr x = New_Diff_Arr [x]" 
 
-definition create_diff_arr_2 where
+definition create_diff_arr_2 ::  "'a::heap \<Rightarrow> 'a list list" where
   "create_diff_arr_2 xs = (let a = New_Diff_Arr [xs]; b = New_Diff_Arr [a] in b)" 
 
-definition create_diff_arr_3 where
+definition create_diff_arr_3 :: "('a::heap) list" where
   "create_diff_arr_3 = (let xs = New_Diff_Arr [] in xs)"
 
-definition create_arr_diff_arr where
+definition create_arr_diff_arr :: "('a::heap) \<Rightarrow> 'a list" where
   "create_arr_diff_arr xs = (let a = New_Arr [xs]; b = Diff_Arr_From_Arr a in b)" 
-
-definition case_tuple where
-  "case_tuple x = (case x of (x1, x2) \<Rightarrow> let c = x2 in x1)"
-
-definition case_nat where
-  "case_nat n = (case n of 
-                        0 \<Rightarrow> let xs = New_Diff_Arr [] in xs 
-                  | Suc n \<Rightarrow> let xs = New_Diff_Arr [] in xs)"
 
 (* HNR Array *)
 
-schematic_goal "hnr (array_assn xs xsi) (?c :: ?'a Heap) ?\<Gamma>' (sequential_1 xs)"
+synth_definition sequential_1_arr is [hnr_rule_arr]: 
+  "hnr (array_assn xs xsi) (\<hole> :: ?'a Heap) ?\<Gamma>' (sequential_1 xs)"
   unfolding sequential_1_def 
   by hnr_arr
 
-schematic_goal "hnr (array_assn xs xsi) (?c :: ?'a Heap) ?\<Gamma>' (sequential_2 xs)"
+synth_definition sequential_2_arr is [hnr_rule_arr]: 
+  "hnr (array_assn xs xsi) (\<hole> :: ?'a Heap) ?\<Gamma>' (sequential_2 xs)"
   unfolding sequential_2_def 
   by hnr_arr
 
-
-schematic_goal "hnr (array_assn xs xsi) (?c :: ?'a Heap) ?\<Gamma>' (return_tuple_1 xs)"
+synth_definition return_tuple_1_arr is [hnr_rule_arr]: 
+  "hnr (array_assn xs xsi) (\<hole> :: ?'a Heap) ?\<Gamma>' (return_tuple_1 xs)"
   unfolding return_tuple_1_def
   by hnr_arr
 
-lemma tuple_simp: "(let x = (a, b) in f x) = (let x1 = a; x2 = b in f (x1, x2))"
-  by simp
- 
-lemma hnr_t:
-  assumes "hnr \<Gamma> pi \<Gamma>' (fst p, snd p)"
-  shows "hnr \<Gamma> pi \<Gamma>' p"
-  using assms 
-  by auto
-
-(* TODO: *)
-schematic_goal "hnr (array_assn xs xsi) (?c :: ?'a Heap) ?\<Gamma>' (return_tuple_4 xs)"
-  unfolding return_tuple_4_def
-  by hnr_arr
-
-lemma hnr_tuple_2: 
-  shows 
-    "hnr 
-      (A a ai * B b bi)
-      (return (ai, bi))
-      (\<lambda> p pi. A (fst p) (fst pi) * B (snd p) (snd pi))
-      (a, b)"
-  apply(rule hnrI)
-  by sep_auto
-
-schematic_goal "hnr (array_assn xs xsi) (?c :: ?'a Heap) ?\<Gamma>' (return_tuple_2 xs)"
+synth_definition return_tuple_2_arr is [hnr_rule_arr]: 
+  "hnr (array_assn xs xsi) (\<hole> :: ?'a Heap) ?\<Gamma>' (return_tuple_2 xs)"
   unfolding return_tuple_2_def
   by hnr_arr
 
 (* Can't work, not linear! *)
-schematic_goal "hnr (array_assn xs xsi) (?c :: ?'a Heap) ?\<Gamma>' (return_tuple_3 xs)"
+synth_definition return_tuple_3_arr is [hnr_rule_arr]: 
+  "hnr (array_assn xs xsi) (\<hole> :: ?'a Heap) ?\<Gamma>' (return_tuple_3 xs)"
   unfolding return_tuple_3_def 
   apply hnr_arr
   oops  
 
+synth_definition return_tuple_4_arr is [hnr_rule_arr]: 
+  "hnr (array_assn xs xsi) (\<hole> :: ?'a Heap) ?\<Gamma>' (return_tuple_4 xs)"
+  unfolding return_tuple_4_def
+  by hnr_arr
+
 (* Can't work, not linear! *)
-schematic_goal "hnr (array_assn xs xsi) (?c :: ?'a Heap) ?\<Gamma>' (not_linear xs)"
+synth_definition not_linear_arr is
+  "hnr (array_assn xs xsi) (\<hole> :: ?'a Heap) ?\<Gamma>' (not_linear xs)"
   unfolding not_linear_def 
   apply hnr_arr
   oops 
 
-schematic_goal "hnr (array_assn xs xsi) (?c :: ?'a Heap) ?\<Gamma>' (if_1 xs)"
+synth_definition if_1_arr is [hnr_rule_arr]:
+  "hnr (array_assn xs xsi) (\<hole> :: ?'a Heap) ?\<Gamma>' (if_1 xs)"
   unfolding if_1_def 
   by hnr_arr
 
-schematic_goal "hnr (array_assn xs xsi) (?c :: ?'a Heap) ?\<Gamma>' (if_2 xs)"
+synth_definition if_2_arr is [hnr_rule_arr]: 
+  "hnr (array_assn xs xsi) (\<hole> :: ?'a Heap) ?\<Gamma>' (if_2 xs)"
   unfolding if_2_def 
   by hnr_arr
 
-schematic_goal "hnr (array_assn xs xsi) (?c :: ?'a Heap) ?\<Gamma>' (if_3 xs)"
+(* 
+  Shouldn't work, not linear! (Or best behavior would be that if something is not 
+  linear it leaves in lists, such that then there automatically diff arrs are put)
+*)
+synth_definition if_3_arr is
+  "hnr (array_assn xs xsi) (\<hole> :: ?'a Heap) ?\<Gamma>' (if_3 xs)"
   unfolding if_3_def 
   by hnr_arr
 
-schematic_goal "hnr (array_assn xs xsi) (?c :: ?'a Heap) ?\<Gamma>' (if_4 xs)"
+synth_definition if_4_arr is [hnr_rule_arr]: 
+  "hnr (array_assn xs xsi) (\<hole> :: ?'a Heap) ?\<Gamma>' (if_4 xs)"
   unfolding if_4_def 
   by hnr_arr
 
-schematic_goal "hnr (array_assn xs xsi) (?c :: ?'a Heap) ?\<Gamma>' (if_5 xs)"
+synth_definition if_5_arr is [hnr_rule_arr]:   
+  "hnr (array_assn xs xsi) (\<hole> :: ?'a Heap) ?\<Gamma>' (if_5 xs)"
   unfolding if_5_def 
   by hnr_arr
 
-(* TODO: There is something wrong here *)
-schematic_goal "hnr (array_assn xs xsi) (?c :: ?'a Heap) ?\<Gamma>' (if_6 xs)"
+(* Shouldn't work, not linear! *)
+synth_definition if_6_arr is 
+  "hnr (array_assn xs xsi) (\<hole> :: ?'a Heap) ?\<Gamma>' (if_6 xs)"
   unfolding if_6_def 
   by hnr_arr
 
-(* TODO: There is something wrong here *)
-schematic_goal "hnr (array_assn xs xsi) (?c :: ?'a Heap) ?\<Gamma>' (if_7 xs)"
+(* TODO: There is something wrong here \<Longrightarrow> I should reconsider the return-fallback  *)
+synth_definition if_7_arr is
+  "hnr (array_assn xs xsi) (\<hole> :: ?'a Heap) ?\<Gamma>' (if_7 xs)"
   unfolding if_7_def 
   by hnr_arr
 
-(* TODO: Why does this work ? *)
-schematic_goal "hnr (array_assn xs xsi) (?c :: ?'a Heap) ?\<Gamma>' (fallback_1 xs)"
-  unfolding fallback_1_def 
+synth_definition tuple_list_arr is [hnr_rule_arr]:
+  "hnr (array_assn xs xsi) (\<hole> :: ?'a Heap) ?\<Gamma>' (tuple_list xs)"
+  unfolding tuple_list_def 
   by hnr_arr
 
-(* TODO *)
-schematic_goal "hnr emp (?c :: ?'a Heap) ?\<Gamma>' (create_list x)"
+synth_definition nested_arr is 
+  "hnr (array_assn xs xsi) (\<hole> :: ?'a Heap) ?\<Gamma>' (nested xs)"
+  unfolding nested_def 
+  by hnr_step_arr+
+
+synth_definition create_list_arr is [hnr_rule_arr]:
+  "hnr emp (\<hole> :: ?'a Heap) ?\<Gamma>' (create_list x)"
   unfolding create_list_def 
   by hnr_arr
 
-(* TODO *)
-schematic_goal "hnr emp (?c :: ?'a Heap) ?\<Gamma>' (create_arr x)"
+synth_definition create_arr_impl is [hnr_rule_arr]:
+  "hnr emp (\<hole> :: ?'a Heap) ?\<Gamma>' (create_arr (xs :: ('a::heap) list))"
   unfolding create_arr_def 
   by hnr_arr
 
-(* TODO *)
-schematic_goal "hnr (id_assn x xi) (?c :: ?'a Heap) ?\<Gamma>' (case_tuple x)"
-  unfolding case_tuple_def
-  by hnr_arr
-
-(* TODO *)
-schematic_goal "hnr (id_assn x xi) (?c :: ?'a Heap) ?\<Gamma>' (case_nat x)"
-  unfolding case_nat_def
+synth_definition create_arr_2_impl is [hnr_rule_arr]:
+  "hnr emp (\<hole> :: ?'a Heap) ?\<Gamma>' (create_arr_2 (x :: 'a :: heap))"
+  unfolding create_arr_2_def 
   by hnr_arr
 
 (* HNR Diff-Array *)
 
-schematic_goal "hnr (master_assn' {(xs, xsi)}) (?c :: ?'a Heap) ?\<Gamma>' (test xs)"
-  unfolding test_def 
-  apply hnr_diff_arr
-  done
-
-schematic_goal "hnr (master_assn' {(xs, xsi)}) (?c :: ?'a Heap) ?\<Gamma>' (sequential_1 xs)"
+synth_definition sequential_1_diff_arr is [hnr_rule_diff_arr]:
+  "hnr (master_assn' (insert (xs, xsi) F)) (\<hole> :: ?'a Heap) ?\<Gamma>' (sequential_1 xs)"
   unfolding sequential_1_def 
   by hnr_diff_arr
 
-schematic_goal "hnr (master_assn' {(xs, xsi)}) (?c :: ?'a Heap) ?\<Gamma>' (sequential_2 xs)"
+synth_definition sequential_2_diff_arr is [hnr_rule_diff_arr]: 
+  "hnr (master_assn' {(xs, xsi)}) (\<hole> :: ?'a Heap) ?\<Gamma>' (sequential_2 xs)"
   unfolding sequential_2_def
-  thm hnr_let
   by hnr_diff_arr
 
-schematic_goal "hnr(master_assn' {(xs, xsi)}) (?c :: ?'a Heap) ?\<Gamma>' (return_tuple_1 xs)"
+synth_definition return_tuple_1_diff_arr is [hnr_rule_diff_arr]: 
+  "hnr(master_assn' {(xs, xsi)}) (\<hole> :: ?'a Heap) ?\<Gamma>' (return_tuple_1 xs)"
   unfolding return_tuple_1_def
   by hnr_diff_arr
 
-(* TODO: Why is there no assn afterwards? *)
-schematic_goal "hnr (master_assn' {(xs, xsi)}) (?c :: ?'a Heap) ?\<Gamma>' (return_tuple_2 xs)"
+synth_definition return_tuple_2_diff_arr is [hnr_rule_diff_arr]:
+  "hnr (master_assn' {(xs, xsi)}) (\<hole> :: ?'a Heap) ?\<Gamma>' (return_tuple_2 xs)"
   unfolding return_tuple_2_def 
   by hnr_diff_arr
-    
-
-find_theorems "hnr _ (return _) _ _ "
-
-
-(* TODO: Why is there no assn afterwards? *)
-schematic_goal "hnr (master_assn' {(xs, xsi)}) (?c :: ?'a Heap) ?\<Gamma>' (return_tuple_3 xs)"
+   
+synth_definition return_tuple_3_diff_arr is [hnr_rule_diff_arr]: 
+  "hnr (master_assn' {(xs, xsi)}) (\<hole> :: ?'a Heap) ?\<Gamma>' (return_tuple_3 xs)"
   unfolding return_tuple_3_def 
   by hnr_diff_arr
 
-schematic_goal "hnr (master_assn' {(xs, xsi)}) (?c :: ?'a Heap) ?\<Gamma>' (not_linear xs)"
+synth_definition return_tuple_4_diff_arr is [hnr_rule_diff_arr]: 
+  "hnr (master_assn' {(xs, xsi)}) (\<hole> :: ?'a Heap) ?\<Gamma>' (return_tuple_4 xs)"
+  unfolding return_tuple_4_def
+  by hnr_diff_arr
+
+synth_definition not_linear_diff_arr is [hnr_rule_diff_arr]:
+  "hnr (master_assn' {(xs, xsi)}) (\<hole> :: ?'a Heap) ?\<Gamma>' (not_linear xs)"
   unfolding not_linear_def 
   by hnr_diff_arr
 
-schematic_goal "hnr (master_assn' {(xs, xsi)}) (?c :: ?'a Heap) ?\<Gamma>' (if_1 xs)"
+synth_definition if_1_diff_arr is [hnr_rule_diff_arr]:
+  "hnr (master_assn' {(xs, xsi)}) (\<hole> :: ?'a Heap) ?\<Gamma>' (if_1 xs)"
   unfolding if_1_def 
   by hnr_diff_arr
 
-schematic_goal "hnr (master_assn' {(xs, xsi)}) (?c :: ?'a Heap) ?\<Gamma>' (if_2 xs)"
+synth_definition if_2_diff_arr is [hnr_rule_diff_arr]:
+  "hnr (master_assn' {(xs, xsi)}) (\<hole> :: ?'a Heap) ?\<Gamma>' (if_2 xs)"
   unfolding if_2_def 
   by hnr_diff_arr
 
-schematic_goal "hnr (master_assn' {(xs, xsi)}) (?c :: ?'a Heap) ?\<Gamma>' (if_3 xs)"
+synth_definition if_3_diff_arr is [hnr_rule_diff_arr]:
+  "hnr (master_assn' {(xs, xsi)}) (\<hole> :: ?'a Heap) ?\<Gamma>' (if_3 xs)"
   unfolding if_3_def 
   by hnr_diff_arr
 
-schematic_goal "hnr (master_assn' {(xs, xsi)}) (?c :: ?'a Heap) ?\<Gamma>' (if_4 xs)"
+synth_definition if_4_diff_arr is [hnr_rule_diff_arr]:
+  "hnr (master_assn' {(xs, xsi)}) (\<hole> :: ?'a Heap) ?\<Gamma>' (if_4 xs)"
   unfolding if_4_def 
   by hnr_diff_arr
 
-schematic_goal "hnr (master_assn' {(xs, xsi)}) (?c :: ?'a Heap) ?\<Gamma>' (if_5 xs)"
+synth_definition if_5_diff_arr is [hnr_rule_diff_arr]:
+  "hnr (master_assn' (insert (xs, xsi) F)) (\<hole> :: ?'a Heap) ?\<Gamma>' (if_5 xs)"
   unfolding if_5_def 
   by hnr_diff_arr
 
-schematic_goal "hnr (master_assn' {(xs, xsi)}) (?c :: ?'a Heap) ?\<Gamma>' (if_6 xs)"
+synth_definition if_6_diff_arr is [hnr_rule_diff_arr]:
+  "hnr (master_assn' {(xs, xsi)}) (\<hole> :: ?'a Heap) ?\<Gamma>' (if_6 xs)"
   unfolding if_6_def 
   by hnr_diff_arr
 
-synth_definition if_7_impl is [hnr_rule_diff_arr]: 
+synth_definition if_7_diff_arr is [hnr_rule_diff_arr]: 
     "hnr (master_assn' (insert (xs, xsi) F)) (\<hole> :: ?'a Heap) ?\<Gamma>' (if_7 xs)"
   unfolding if_7_def   
-  apply hnr_diff_arr
-  done
+  by hnr_diff_arr
 
-print_theorems
+synth_definition tuple_list_diff_arr is [hnr_rule_diff_arr]:
+  "hnr (master_assn' {(xs, xsi)}) (\<hole> :: ?'a Heap) ?\<Gamma>' (tuple_list xs)"
+  unfolding tuple_list_def 
+  by hnr_diff_arr
 
-thm hnr_rule_diff_arr
-
-schematic_goal "hnr (master_assn' (insert (xs, xsi) F)) (?c :: ?'a Heap) ?\<Gamma>' (test_2 xs)"
-  unfolding test_2_def
-  apply hnr_diff_arr
-  done
+synth_definition nested_diff_arr is 
+  "hnr (master_assn' {(xs, xsi)}) (\<hole> :: ?'a Heap) ?\<Gamma>' (nested xs)"
+  unfolding nested_def 
+  by hnr_diff_arr
 
 (* TODO: *)
 schematic_goal "hnr (master_assn' {(xs, xsi)}) (?c :: ?'a Heap) ?\<Gamma>' (fallback_1 xs)"
@@ -334,16 +329,15 @@ schematic_goal "hnr emp (?c :: ?'a Heap) ?\<Gamma>' (create_list x)"
   unfolding create_list_def 
   by hnr_diff_arr
 
-(* TODO: Doesn't seem to work correctly anymore *)
 schematic_goal "hnr emp (?c :: ?'a Heap) ?\<Gamma>' (create_diff_arr_empty)"
   unfolding create_diff_arr_empty_def 
   by hnr_diff_arr
 
-(* TODO: Doesn't seem to work correctly anymore *)
 schematic_goal "hnr emp (?c :: ?'a Heap) ?\<Gamma>' (create_diff_arr x)"
   unfolding create_diff_arr_def 
   by hnr_diff_arr
 
+(* TODO: Nested lists *)
 schematic_goal "hnr emp (?c :: ?'a Heap) ?\<Gamma>' (create_diff_arr_2 x)"
   unfolding create_diff_arr_2_def 
   by hnr_diff_arr
@@ -352,19 +346,11 @@ schematic_goal "hnr emp (?c :: ?'a Heap) ?\<Gamma>' (create_diff_arr_3)"
   unfolding create_diff_arr_3_def 
   by hnr_diff_arr
 
-(* TODO: This worked before ^^ - Do I need a combined operator? *)
+(* TODO: Do I need a combined operator? *)
 schematic_goal "hnr emp (?c :: ?'a Heap) ?\<Gamma>' (create_arr_diff_arr x)"
   unfolding create_arr_diff_arr_def 
-  sorry
-
-schematic_goal "hnr (id_assn x xi) (?c :: ?'a Heap) ?\<Gamma>' (case_tuple x)"
-  unfolding case_tuple_def
+  apply hnr_arr
   by hnr_diff_arr
-
-schematic_goal "hnr (id_assn x xi) (?c :: ?'a Heap) ?\<Gamma>' (case_nat x)"
-  unfolding case_nat_def
-  by hnr_diff_arr
-
 
 export_code array_nth_safe array_update_safe in SML_imp
 
